

De Morgan: $\neg(p \wedge q) \vdash (\neg p \vee \neg q)$. Proof:

1	$\neg(p \wedge q)$	
2	$\neg(\neg p \vee \neg q)$	
3	$\neg p$	
4	$(\neg p \vee \neg q)$	$\vee I \quad 3$
5	\perp	$\perp I \quad 2, 4$
6	$\neg\neg p$	$\neg I \quad 3 - 5$
7	p	$\neg E \quad 6$
8	$\neg q$	
9	$(\neg p \vee \neg q)$	$\vee I \quad 8$
10	\perp	$\perp I \quad 2, 9$
11	$\neg\neg q$	$\neg I \quad 8 - 10$
12	q	$\neg E \quad 11$
13	$(p \wedge q)$	$\wedge I \quad 7, 12$
14	\perp	$\perp I \quad 1, 13$
15	$\neg\neg(\neg p \vee \neg q)$	$\neg I \quad 2, 14$
16	$(\neg p \vee \neg q)$	$\neg E \quad 15$

Done!